testdata/modules/crossmod_missing/main.cue
@@ -1,0 +1,5 @@
+package main
+
+import "gone.example/lib"
+
+out: lib.#X
