testdata/modules/crossmod_transitive/main.cue
@@ -1,0 +1,8 @@
+package main
+
+import "mid.example/lib"
+
+out: lib.#Box & {
+	tag: "outer"
+	inner: {value: 7}
+}
