testdata/modules/crossmod_vendor/main.cue
@@ -1,0 +1,8 @@
+package main
+
+import "lib.example/defs"
+
+out: defs.#Widget & {
+	size:  5
+	label: "vend"
+}
